Weidenbach_Book/CDCL_Two_Watched_Literals_List_Watched_Init_Trail_Code.thy
@@ -2,50 +2,6 @@ theory CDCL_Two_Watched_Literals_List_Watched_Init_Trail_Code
 imports CDCL_Two_Watched_Literals_List_Watched_Trail_Code
 begin
 
-definition init_dt_step_wl :: \<open>uint32 list \<Rightarrow> nat clause_l \<Rightarrow> nat twl_st_wl \<Rightarrow> (nat twl_st_wl) nres\<close> where
-  \<open>init_dt_step_wl N\<^sub>0 C S = do {
-     let (M, N, U, D, NP, UP, Q, WS) = S in
-     case D of
-      None \<Rightarrow>
-      if length C = 1
-      then do {
-        ASSERT (no_dup M);
-        ASSERT (C \<noteq> []);
-        let L = hd C;
-        ASSERT(L \<in> snd ` twl_array_code_ops.D\<^sub>0 N\<^sub>0);
-        let val_L = valued M L;
-        if val_L = None
-        then do {RETURN (Propagated L 0 # M, N, U, None, add_mset {#L#} NP, UP, add_mset (-L) Q, WS)}
-        else
-          if val_L = Some True
-          then do {RETURN (M, N, U, None, add_mset {#L#} NP, UP, Q, WS)}
-          else do {RETURN (M, N, U, Some (mset C), add_mset {#L#} NP, UP, {#}, WS)}
-        }
-      else do {
-        ASSERT(C \<noteq> []);
-        ASSERT(tl C \<noteq> []);
-        ASSERT(hd C \<in> snd ` twl_array_code_ops.D\<^sub>0 N\<^sub>0);
-        ASSERT(hd (tl C) \<in> snd ` twl_array_code_ops.D\<^sub>0 N\<^sub>0);
-        let U = length N;
-        let WS = WS((hd C) := WS (hd C) @ [U]);
-        let WS = WS((hd (tl C)) := WS (hd (tl C)) @ [U]);
-        RETURN (M, N @ [op_array_of_list C], U, None, NP, UP, Q, WS)}
-    | Some D \<Rightarrow>
-      if length C = 1
-      then do {
-        ASSERT (C \<noteq> []);
-        let L = hd C;
-        RETURN (M, N, U, Some D, add_mset {#L#} NP, UP, {#}, WS)}
-      else do {
-        ASSERT(C \<noteq> []);
-        ASSERT(tl C \<noteq> []);
-        ASSERT(hd C \<in> snd ` twl_array_code_ops.D\<^sub>0 N\<^sub>0);
-        ASSERT(hd (tl C) \<in> snd ` twl_array_code_ops.D\<^sub>0 N\<^sub>0);
-        let U = length N;
-        let WS = WS(hd C := WS (hd C) @ [U]);
-        let WS = WS((hd (tl C)) := WS (hd (tl C)) @ [U]);
-        RETURN (M, N @ [op_array_of_list C], U, Some D, NP, UP, {#}, WS)}
-  }\<close>
 
 definition arl_of_list_raa :: "'a::heap list \<Rightarrow> ('a array_list) Heap" where
   \<open>arl_of_list_raa xs = do {
@@ -77,13 +33,61 @@ declare twl_array_code.append_el_aa_hnr[sepref_fr_rules]
 declare twl_array_code.valued_trail_code_valued_refine_code[sepref_fr_rules]
   twl_array_code.cons_trail_Propagated_tr_code_cons_trail_Propagated_tr[sepref_fr_rules]
 
-sepref_thm (in twl_array_code) init_dt_step_wl_code
-  is \<open>uncurry2 init_dt_step_wl\<close>
-  :: \<open>[\<lambda>((N, _), _). N = N\<^sub>0]\<^sub>a
-       (list_assn uint32_assn)\<^sup>k *\<^sub>a (list_assn unat_lit_assn)\<^sup>d *\<^sub>a twl_st_l_trail_assn\<^sup>d \<rightarrow>
+context twl_array_code
+begin
+
+definition init_dt_step_wl :: \<open>nat clause_l \<Rightarrow> nat twl_st_wl \<Rightarrow> (nat twl_st_wl) nres\<close> where
+  \<open>init_dt_step_wl C S = do {
+     let (M, N, U, D, NP, UP, Q, WS) = S in
+     case D of
+       None \<Rightarrow>
+         if length C = 1
+         then do {
+           ASSERT (no_dup M);
+           ASSERT (C \<noteq> []);
+           let L = hd C;
+           ASSERT(L \<in> snd ` D\<^sub>0);
+           let val_L = valued M L;
+           if val_L = None
+           then do {RETURN (Propagated L 0 # M, N, U, None, add_mset {#L#} NP, UP, add_mset (-L) Q, WS)}
+           else
+             if val_L = Some True
+             then do {RETURN (M, N, U, None, add_mset {#L#} NP, UP, Q, WS)}
+             else do {RETURN (M, N, U, Some (mset C), add_mset {#L#} NP, UP, {#}, WS)}
+           }
+         else do {
+           ASSERT(C \<noteq> []);
+           ASSERT(tl C \<noteq> []);
+           ASSERT(hd C \<in> snd ` D\<^sub>0);
+           ASSERT(hd (tl C) \<in> snd ` D\<^sub>0);
+           let U = length N;
+           let WS = WS((hd C) := WS (hd C) @ [U]);
+           let WS = WS((hd (tl C)) := WS (hd (tl C)) @ [U]);
+           RETURN (M, N @ [op_array_of_list C], U, None, NP, UP, Q, WS)}
+    | Some D \<Rightarrow>
+        if length C = 1
+        then do {
+          ASSERT (C \<noteq> []);
+          let L = hd C;
+          RETURN (M, N, U, Some D, add_mset {#L#} NP, UP, {#}, WS)}
+        else do {
+          ASSERT(C \<noteq> []);
+          ASSERT(tl C \<noteq> []);
+          ASSERT(hd C \<in> snd ` D\<^sub>0);
+          ASSERT(hd (tl C) \<in> snd ` D\<^sub>0);
+          let U = length N;
+          let WS = WS(hd C := WS (hd C) @ [U]);
+          let WS = WS((hd (tl C)) := WS (hd (tl C)) @ [U]);
+          RETURN (M, N @ [op_array_of_list C], U, Some D, NP, UP, {#}, WS)}
+  }\<close>
+
+sepref_register init_dt_step_wl
+sepref_thm init_dt_step_wl_code
+  is \<open>uncurry (PR_CONST init_dt_step_wl)\<close>
+  :: \<open>(list_assn unat_lit_assn)\<^sup>d *\<^sub>a twl_st_l_trail_assn\<^sup>d \<rightarrow>\<^sub>a
        twl_st_l_trail_assn\<close>
   supply valued_None_undefined_lit[simp]
-  unfolding init_dt_step_wl_def twl_st_l_trail_assn_def lms_fold_custom_empty
+  unfolding init_dt_step_wl_def twl_st_l_trail_assn_def lms_fold_custom_empty PR_CONST_def
   unfolding watched_app_def[symmetric]
   unfolding nth_rll_def[symmetric] find_unwatched'_find_unwatched[symmetric]
   unfolding lms_fold_custom_empty swap_ll_def[symmetric]
@@ -95,49 +99,49 @@ sepref_thm (in twl_array_code) init_dt_step_wl_code
 
 concrete_definition (in -) init_dt_step_wl_code
   uses "twl_array_code.init_dt_step_wl_code.refine_raw"
-  is "(uncurry2 ?f,_)\<in>_"
+  is "(uncurry ?f,_)\<in>_"
 
 prepare_code_thms (in -) init_dt_step_wl_code_def
 
-lemmas (in twl_array_code) init_dt_step_wl_code_refine[sepref_fr_rules] =
-  init_dt_step_wl_code.refine[sepref_fr_rules, OF twl_array_code_axioms]
+lemmas init_dt_step_wl_code_refine[sepref_fr_rules] =
+  init_dt_step_wl_code.refine[OF twl_array_code_axioms]
 
 definition init_dt_wl where
-  \<open>init_dt_wl N CS S = nfoldli CS (\<lambda>_. True) (init_dt_step_wl N) S\<close>
+  \<open>init_dt_wl CS S = nfoldli CS (\<lambda>_. True) (init_dt_step_wl) S\<close>
 
-sepref_thm (in twl_array_code) init_dt_wl_code
-  is \<open>uncurry2 init_dt_wl\<close>
-  :: \<open>[\<lambda>((N, _), _). N = N\<^sub>0]\<^sub>a
-       (list_assn uint32_assn)\<^sup>k *\<^sub>a (list_assn (list_assn unat_lit_assn))\<^sup>d *\<^sub>a twl_st_l_trail_assn\<^sup>d \<rightarrow>
+sepref_register init_dt_wl
+
+sepref_thm init_dt_wl_code
+  is \<open>uncurry (PR_CONST init_dt_wl)\<close>
+  :: \<open>(list_assn (list_assn unat_lit_assn))\<^sup>d *\<^sub>a twl_st_l_trail_assn\<^sup>d \<rightarrow>\<^sub>a
        twl_st_l_trail_assn\<close>
-  unfolding init_dt_wl_def
+  unfolding init_dt_wl_def PR_CONST_def
   supply [[goals_limit = 1]]
   by sepref
 
 concrete_definition (in -) init_dt_wl_code
   uses "twl_array_code.init_dt_wl_code.refine_raw"
-  is "(uncurry2 ?f,_)\<in>_"
+  is "(uncurry ?f,_)\<in>_"
 
 prepare_code_thms (in -) init_dt_wl_code_def
 
-lemmas (in twl_array_code)init_dt_wl_code_refine[sepref_fr_rules] =
-  init_dt_wl_code.refine[of N\<^sub>0, OF twl_array_code_axioms,
+lemmas init_dt_wl_code_refine[sepref_fr_rules] =
+  init_dt_wl_code.refine[OF twl_array_code_axioms,
     unfolded twl_array_code_ops.twl_st_l_trail_assn_def]
 
-term nat_lit_assn
-term nat_lit_rel
-  term \<open>hs.assn\<close>
-definition nat_lit_list_hm_ref_rel :: "(('a set \<times> 'a literal list) \<times> 'a literal list) set" where
-  \<open>nat_lit_list_hm_ref_rel = {((s, xs), l). l = xs \<and> s = atm_of ` set l}\<close>
+end
+
+definition nat_lit_list_hm_ref_rel :: "(('a set \<times> 'a list) \<times> 'a list) set" where
+  \<open>nat_lit_list_hm_ref_rel = {((s, xs), l). l = xs \<and> s = set l}\<close>
 
 abbreviation nat_lit_lits_init_ref_assn where
-  \<open>nat_lit_lits_init_ref_assn \<equiv> hs.assn uint32_nat_assn *assn list_assn unat_lit_assn\<close>
+  \<open>nat_lit_lits_init_ref_assn \<equiv> hs.assn uint32_nat_assn *assn list_assn uint32_nat_assn\<close>
 
 abbreviation nat_lit_list_hm_assn where
   \<open>nat_lit_list_hm_assn \<equiv> hr_comp nat_lit_lits_init_ref_assn nat_lit_list_hm_ref_rel\<close>
 
-definition in_map_atm_of :: "'a \<Rightarrow> 'a literal list \<Rightarrow> bool" where
-  \<open>in_map_atm_of L N \<longleftrightarrow> L \<in> set (map atm_of N)\<close>
+definition in_map_atm_of :: "'a \<Rightarrow> 'a list \<Rightarrow> bool" where
+  \<open>in_map_atm_of L N \<longleftrightarrow> L \<in> set N\<close>
 
 sepref_definition nat_lit_lits_init_assn_assn_in
   is \<open>uncurry (RETURN oo (\<lambda>L (s, xs). L \<in> s))\<close>
@@ -150,22 +154,23 @@ lemma nat_lit_lits_init_assn_ref_in:
   by (intro frefI nres_relI) (auto simp: nat_lit_list_hm_ref_rel_def in_map_atm_of_def)
 
 sepref_definition nat_lit_lits_init_assn_assn_prepend
-  is \<open>uncurry (RETURN oo (\<lambda>L (s, xs). (insert (atm_of L) s, L # xs)))\<close>
-  :: \<open>unat_lit_assn\<^sup>k *\<^sub>a nat_lit_lits_init_ref_assn\<^sup>d \<rightarrow>\<^sub>a nat_lit_lits_init_ref_assn\<close>
+  is \<open>uncurry (RETURN oo (\<lambda>L (s, xs). (insert L s, L # xs)))\<close>
+  :: \<open>uint32_nat_assn\<^sup>k *\<^sub>a nat_lit_lits_init_ref_assn\<^sup>d \<rightarrow>\<^sub>a nat_lit_lits_init_ref_assn\<close>
   by sepref
 
 lemma nat_lit_lits_init_assn_ref_list_prepend:
-  \<open>(uncurry (RETURN oo (\<lambda>L (s, xs). (insert (atm_of L) s, L # xs))), uncurry (RETURN oo op_list_prepend)) \<in>
+  \<open>(uncurry (RETURN oo (\<lambda>L (s, xs). (insert L s, L # xs))), 
+      uncurry (RETURN oo op_list_prepend)) \<in>
     Id \<times>\<^sub>r nat_lit_list_hm_ref_rel \<rightarrow>\<^sub>f \<langle>nat_lit_list_hm_ref_rel\<rangle>nres_rel\<close>
   by (intro frefI nres_relI) (auto simp: nat_lit_list_hm_ref_rel_def in_map_atm_of_def)
 
 lemma nat_lit_lits_init_assn_assn_prepend[sepref_fr_rules]:
   \<open>(uncurry nat_lit_lits_init_assn_assn_prepend, uncurry (RETURN \<circ>\<circ> op_list_prepend))
-      \<in> unat_lit_assn\<^sup>k *\<^sub>a nat_lit_list_hm_assn\<^sup>d \<rightarrow>\<^sub>a nat_lit_list_hm_assn\<close>
+      \<in> uint32_nat_assn\<^sup>k *\<^sub>a nat_lit_list_hm_assn\<^sup>d \<rightarrow>\<^sub>a nat_lit_list_hm_assn\<close>
   using nat_lit_lits_init_assn_assn_prepend.refine[FCOMP nat_lit_lits_init_assn_ref_list_prepend] .
 
 lemma nat_lit_lits_init_assn_assn_id[sepref_fr_rules]:
-  \<open>(return o snd, RETURN o id) \<in> nat_lit_list_hm_assn\<^sup>d \<rightarrow>\<^sub>a list_assn unat_lit_assn\<close>
+  \<open>(return o snd, RETURN o id) \<in> nat_lit_list_hm_assn\<^sup>d \<rightarrow>\<^sub>a list_assn uint32_nat_assn\<close>
   by sepref_to_hoare (sep_auto simp: nat_lit_list_hm_ref_rel_def hr_comp_def)
 
 lemma in_map_atm_of_hnr[sepref_fr_rules]:
@@ -174,57 +179,56 @@ lemma in_map_atm_of_hnr[sepref_fr_rules]:
   using nat_lit_lits_init_assn_assn_in.refine[FCOMP nat_lit_lits_init_assn_ref_in] .
 
 
-definition extract_lits_cls :: \<open>'a clause_l \<Rightarrow> 'a literal list \<Rightarrow> 'a literal list\<close> where
-  \<open>extract_lits_cls C N\<^sub>0 = fold (\<lambda>L N\<^sub>0. if atm_of L \<in> set (map atm_of N\<^sub>0) then N\<^sub>0 else -L # N\<^sub>0) C N\<^sub>0\<close>
+definition extract_atms_cls :: \<open>'a clause_l \<Rightarrow> 'a list \<Rightarrow> 'a list\<close> where
+  \<open>extract_atms_cls C N\<^sub>0 = fold (\<lambda>L N\<^sub>0. if atm_of L \<in> set N\<^sub>0 then N\<^sub>0 else atm_of L # N\<^sub>0) C N\<^sub>0\<close>
 
-sepref_definition extract_lits_cls_imp
-  is \<open>uncurry (RETURN oo extract_lits_cls)\<close>
+sepref_definition extract_atms_cls_imp
+  is \<open>uncurry (RETURN oo extract_atms_cls)\<close>
   :: \<open>(list_assn unat_lit_assn)\<^sup>k *\<^sub>a nat_lit_list_hm_assn\<^sup>d \<rightarrow>\<^sub>a nat_lit_list_hm_assn\<close>
-  unfolding extract_lits_cls_def in_map_atm_of_def[symmetric]
+  unfolding extract_atms_cls_def in_map_atm_of_def[symmetric]
   by sepref
 
-declare extract_lits_cls_imp.refine[sepref_fr_rules]
+declare extract_atms_cls_imp.refine[sepref_fr_rules]
 
-definition extract_lits_clss:: \<open>'a clauses_l \<Rightarrow> 'a literal list \<Rightarrow> 'a literal list\<close>  where
-  \<open>extract_lits_clss N N\<^sub>0 = fold extract_lits_cls N N\<^sub>0\<close>
+definition extract_atms_clss:: \<open>'a clauses_l \<Rightarrow> 'a list \<Rightarrow> 'a list\<close>  where
+  \<open>extract_atms_clss N N\<^sub>0 = fold extract_atms_cls N N\<^sub>0\<close>
 
-sepref_definition extract_lits_clss_imp
-  is \<open>uncurry (RETURN oo extract_lits_clss)\<close>
+sepref_definition extract_atms_clss_imp
+  is \<open>uncurry (RETURN oo extract_atms_clss)\<close>
   :: \<open>(list_assn (list_assn unat_lit_assn))\<^sup>k *\<^sub>a nat_lit_list_hm_assn\<^sup>d \<rightarrow>\<^sub>a nat_lit_list_hm_assn\<close>
-  unfolding extract_lits_clss_def in_map_atm_of_def[symmetric]
+  unfolding extract_atms_clss_def in_map_atm_of_def[symmetric]
   by sepref
 
-lemma id_extract_lits_clss: \<open>extract_lits_clss = (\<lambda>a b. id (extract_lits_clss a b))\<close>
+lemma id_extract_atms_clss: \<open>extract_atms_clss = (\<lambda>a b. id (extract_atms_clss a b))\<close>
   by auto
 
-sepref_definition extract_lits_clss_imp_list_assn
-  is \<open>uncurry (RETURN oo extract_lits_clss)\<close>
-  :: \<open>(list_assn (list_assn unat_lit_assn))\<^sup>k *\<^sub>a nat_lit_list_hm_assn\<^sup>d \<rightarrow>\<^sub>a list_assn unat_lit_assn\<close>
-  supply extract_lits_clss_imp.refine[sepref_fr_rules]
-  apply (rewrite at \<open>extract_lits_clss\<close> id_extract_lits_clss)
+sepref_definition extract_atms_clss_imp_list_assn
+  is \<open>uncurry (RETURN oo extract_atms_clss)\<close>
+  :: \<open>(list_assn (list_assn unat_lit_assn))\<^sup>k *\<^sub>a nat_lit_list_hm_assn\<^sup>d \<rightarrow>\<^sub>a list_assn uint32_nat_assn\<close>
+  supply extract_atms_clss_imp.refine[sepref_fr_rules]
+  apply (rewrite at \<open>extract_atms_clss\<close> id_extract_atms_clss)
   by sepref
 
 definition op_extract_list_empty where
   \<open>op_extract_list_empty = []\<close>
 
-lemma extract_lits_clss_imp_empty_rel:
+lemma extract_atms_clss_imp_empty_rel:
   \<open>(uncurry0 (RETURN ({}, [])), uncurry0 (RETURN op_extract_list_empty)) \<in>
      unit_rel \<rightarrow>\<^sub>f \<langle>nat_lit_list_hm_ref_rel\<rangle> nres_rel\<close>
   by (intro frefI nres_relI) (auto simp: nat_lit_list_hm_ref_rel_def op_extract_list_empty_def)
 
-sepref_definition extract_lits_clss_imp_empty_assn
+sepref_definition extract_atms_clss_imp_empty_assn
   is \<open>uncurry0 (RETURN ({}, []))\<close>
   :: \<open>unit_assn\<^sup>k \<rightarrow>\<^sub>a nat_lit_lits_init_ref_assn\<close>
   unfolding hs.fold_custom_empty HOL_list.fold_custom_empty
   by sepref
 
-
-lemma extract_lits_clss_imp_empty_assn[sepref_fr_rules]:
-  \<open>(uncurry0 extract_lits_clss_imp_empty_assn, uncurry0 (RETURN op_extract_list_empty))
+lemma extract_atms_clss_imp_empty_assn[sepref_fr_rules]:
+  \<open>(uncurry0 extract_atms_clss_imp_empty_assn, uncurry0 (RETURN op_extract_list_empty))
     \<in> unit_assn\<^sup>k \<rightarrow>\<^sub>a nat_lit_list_hm_assn\<close>
-  using extract_lits_clss_imp_empty_assn.refine[FCOMP extract_lits_clss_imp_empty_rel] .
+  using extract_atms_clss_imp_empty_assn.refine[FCOMP extract_atms_clss_imp_empty_rel] .
 
-declare extract_lits_clss_imp_list_assn.refine[sepref_fr_rules]
+declare extract_atms_clss_imp_list_assn.refine[sepref_fr_rules]
 declare atm_of_hnr[sepref_fr_rules]
 
 sepref_definition find_first_eq_map_atm_of_code
@@ -248,95 +252,89 @@ proof -
     using find_first_eq_map_atm_of_code.refine[FCOMP 1] .
 qed
 
-definition extract_lits_cls' :: \<open>'a clause_l \<Rightarrow> 'a literal list \<Rightarrow> 'a literal list\<close> where
-  \<open>extract_lits_cls' C N\<^sub>0 =
-     fold (\<lambda>L N\<^sub>0. let i = index (map atm_of N\<^sub>0) (atm_of L) in if i < length N\<^sub>0 then N\<^sub>0 else -L # N\<^sub>0) C N\<^sub>0\<close>
+(* TODO Move *)
+lemma all_lits_of_mm_empty[simp]: \<open>all_lits_of_mm {#} = {#}\<close>
+  by (auto simp: all_lits_of_mm_def)
 
-sepref_definition extract_lits_cls_code
-  is \<open>uncurry (RETURN oo extract_lits_cls')\<close>
-  :: \<open>(list_assn unat_lit_assn)\<^sup>d *\<^sub>a (list_assn unat_lit_assn)\<^sup>d \<rightarrow>\<^sub>a (list_assn unat_lit_assn)\<close>
-  unfolding extract_lits_cls'_def twl_array_code_ops.twl_st_l_trail_assn_def lms_fold_custom_empty
-  unfolding watched_app_def[symmetric]
-  unfolding nth_rll_def[symmetric] find_unwatched'_find_unwatched[symmetric]
-  unfolding lms_fold_custom_empty swap_ll_def[symmetric]
-  unfolding twl_array_code_ops.append_update_def[symmetric] index_atm_of_def[symmetric]
-  supply [[goals_limit = 1]]
-  by sepref
+lemma all_lits_of_m_empty[simp]: \<open>all_lits_of_m {#} = {#}\<close>
+  by (auto simp: all_lits_of_m_def)
+(* End Move *)
 
-declare extract_lits_cls_code.refine[sepref_fr_rules]
+lemma extract_atms_cls_Cons:
+  \<open>extract_atms_cls (L # C) N\<^sub>0 = extract_atms_cls C (if atm_of L \<in> set N\<^sub>0 then N\<^sub>0 else atm_of L # N\<^sub>0)\<close>
+  unfolding extract_atms_cls_def fold.simps by simp
 
-lemma extract_lits_cls'_extract_lits_cls: \<open>extract_lits_cls' = extract_lits_cls\<close>
-proof -
-  have [simp]: \<open>(\<lambda>L N\<^sub>0. if index (map atm_of N\<^sub>0) (atm_of L) < length N\<^sub>0 then N\<^sub>0 else -L # N\<^sub>0) =
-      (\<lambda>L N\<^sub>0. if atm_of L \<in> atm_of ` set N\<^sub>0 then N\<^sub>0 else -L # N\<^sub>0)\<close>
-    by (intro ext) (auto simp: extract_lits_cls'_def extract_lits_cls_def)
-  then show ?thesis
-    by (intro ext) (auto simp: extract_lits_cls'_def extract_lits_cls_def)
-qed
+lemma extract_atms_cls_Nil[simp]:
+  \<open>extract_atms_cls [] N\<^sub>0 = N\<^sub>0\<close>
+  unfolding extract_atms_cls_def fold.simps by simp
 
-sepref_definition extract_lits_clss_code
-  is \<open>uncurry (RETURN oo extract_lits_clss)\<close>
-  :: \<open>(list_assn (list_assn unat_lit_assn))\<^sup>d *\<^sub>a (list_assn unat_lit_assn)\<^sup>d \<rightarrow>\<^sub>a (list_assn unat_lit_assn)\<close>
-  unfolding extract_lits_clss_def extract_lits_cls'_extract_lits_cls[symmetric]
-  by sepref
+lemma extract_atms_clss_Cons[simp]:
+  \<open>extract_atms_clss (C # Cs) N = extract_atms_clss Cs (extract_atms_cls C N)\<close>
+  by (simp add: extract_atms_clss_def)
 
-declare extract_lits_clss_code.refine[sepref_fr_rules]
 
-lemma lits_of_atms_of_mm_empty[simp]: \<open>lits_of_atms_of_mm {#} = {#}\<close>
-  by (auto simp: lits_of_atms_of_mm_def)
+definition (in -) all_lits_of_atms_m :: \<open>'a multiset \<Rightarrow> 'a clause\<close> where
+ \<open>all_lits_of_atms_m N = poss N + negs N\<close>
 
-lemma lits_of_atms_of_m_empty[simp]: \<open>lits_of_atms_of_m {#} = {#}\<close>
-  by (auto simp: lits_of_atms_of_m_def)
+definition (in -) all_lits_of_atms_mm :: \<open>'a multiset multiset \<Rightarrow> 'a clause\<close> where
+ \<open>all_lits_of_atms_mm N = poss (\<Union># N) + negs (\<Union># N)\<close>
 
-lemma extract_lits_cls_Cons:
-  \<open>extract_lits_cls (L # C) N\<^sub>0 = extract_lits_cls C (if atm_of L \<in> atms_of (mset N\<^sub>0) then N\<^sub>0 else -L # N\<^sub>0)\<close>
-  unfolding extract_lits_cls_def fold.simps by simp
+lemma all_lits_of_atms_mm_all_lits_of_mm:
+  \<open>all_lits_of_atms_mm N = all_lits_of_mm (poss `# N)\<close>
+  unfolding all_lits_of_atms_mm_def all_lits_of_mm_def
+  by (induction N) auto
 
-lemma extract_lits_cls_Nil[simp]:
-  \<open>extract_lits_cls [] N\<^sub>0 = N\<^sub>0\<close>
-  unfolding extract_lits_cls_def fold.simps by simp
+lemma all_lits_of_atms_m_all_lits_of_m:
+  \<open>all_lits_of_atms_m N = all_lits_of_m (poss N)\<close>
+  unfolding all_lits_of_atms_m_def all_lits_of_m_def
+  by (induction N) auto
 
-lemma extract_lits_clss_Cons[simp]:
-  \<open>extract_lits_clss (C # Cs) N = extract_lits_clss Cs (extract_lits_cls C N)\<close>
-  by (simp add: extract_lits_clss_def)
-
-lemma lits_of_atms_of_m_extract_lits_cls: \<open>set_mset (lits_of_atms_of_m (mset (extract_lits_cls C N\<^sub>0))) =
-   set_mset (lits_of_atms_of_m (mset C) + lits_of_atms_of_m (mset N\<^sub>0))\<close>
+lemma all_lits_of_m_extract_atms_cls: \<open>set_mset (all_lits_of_atms_m (mset (extract_atms_cls C N\<^sub>0))) =
+   set_mset (all_lits_of_m (mset C) + all_lits_of_atms_m (mset N\<^sub>0))\<close>
   apply (induction C arbitrary: N\<^sub>0)
   subgoal by simp
-  subgoal by (auto simp add: extract_lits_cls_Cons lits_of_atms_of_m_add_mset
-        in_lits_of_atms_of_m_ain_atms_of_iff insert_absorb)
+  subgoal by (auto simp add: extract_atms_cls_Cons all_lits_of_m_add_mset uminus_literal_def
+        in_all_lits_of_m_ain_atms_of_iff insert_absorb all_lits_of_atms_m_all_lits_of_m)
   done
 
 lemma nat_of_lit_upperN_nat_of_lit_uminus_upperN:
   \<open>nat_of_lit (-L) < upperN \<longleftrightarrow> nat_of_lit L < upperN\<close>
   by (cases L) (auto simp: upperN_def)
 
-lemma in_extract_lits_clsD:
-  \<open>L \<in> set (extract_lits_cls C N\<^sub>0) \<Longrightarrow> L \<in> set C \<union> set N\<^sub>0 \<or> -L \<in> set C \<union> set N\<^sub>0\<close>
+lemma in_extract_atms_clsD:
+  \<open>L \<in> set (extract_atms_cls C N\<^sub>0) \<Longrightarrow> L \<in> atms_of_s (set C) \<union> set N\<^sub>0\<close>
   apply (induction C arbitrary: N\<^sub>0)
   subgoal by auto
   subgoal premises IH for L' C N\<^sub>0
-    using IH(1)[of \<open>(if atm_of L' \<in> atm_of ` set N\<^sub>0 then N\<^sub>0 else -L' # N\<^sub>0)\<close>] IH(2)
-    by (auto simp: extract_lits_cls_def split: if_splits)
+    using IH(1)[of \<open>(if atm_of L' \<in> set N\<^sub>0 then N\<^sub>0 else atm_of L' # N\<^sub>0)\<close>] IH(2)
+    by (auto simp: extract_atms_cls_def split: if_splits)
   done
 
-lemma in_extract_lits_clssD:
-  \<open>L \<in> set (extract_lits_clss C N\<^sub>0) \<Longrightarrow> L \<in> \<Union>(set`set C) \<union> set N\<^sub>0 \<or> -L \<in> \<Union>(set`set C) \<union> set N\<^sub>0\<close>
+lemma in_extract_atms_clssD:
+  fixes N\<^sub>0 :: \<open>'a list\<close>
+  shows
+    \<open>L \<in> set (extract_atms_clss C N\<^sub>0) \<Longrightarrow> L \<in> atms_of_s (\<Union>(set`set C)) \<union> set N\<^sub>0\<close>
   apply (induction C arbitrary: N\<^sub>0)
-  subgoal by (auto simp: extract_lits_clss_def)
+  subgoal by (auto simp: extract_atms_clss_def)
   subgoal premises IH for L' C N\<^sub>0
-    using IH(1)[of \<open>(extract_lits_cls L' N\<^sub>0)\<close>] IH(2)
-    by (auto simp: extract_lits_clss_def split: if_splits dest: in_extract_lits_clsD)
+    using IH(1)[of \<open>(extract_atms_cls L' N\<^sub>0)\<close>] IH(2)
+    by (auto simp: extract_atms_clss_def split: if_splits dest: in_extract_atms_clsD)
   done
 
-lemma is_N\<^sub>1_extract_lits_clss:
-  assumes upper: \<open>\<forall>L \<in> set N\<^sub>0. nat_of_lit L < upperN\<close>
+definition N\<^sub>0_of_atms where
+\<open>N\<^sub>0_of_atms N = map (uint32_of_nat o (op * 2)) N\<close>
+
+lemma is_N\<^sub>1_extract_atms_clss:
+  assumes upper: \<open>\<forall>L \<in> set N\<^sub>0. L < upperN div 2\<close>
   assumes upperN: \<open>\<forall>C \<in> set N. \<forall>L \<in> set C. nat_of_lit L < upperN\<close>
   shows
-   \<open>twl_array_code_ops.is_N\<^sub>1 (map (uint32_of_nat o nat_of_lit) (extract_lits_clss N N\<^sub>0))
-     (lits_of_atms_of_mm (mset `# mset N) + lits_of_atms_of_m (mset N\<^sub>0))\<close>
+   \<open>twl_array_code_ops.is_N\<^sub>1 (N\<^sub>0_of_atms (extract_atms_clss N N\<^sub>0))
+     (all_lits_of_mm (mset `# mset N) + all_lits_of_atms_m (mset N\<^sub>0))\<close>
 proof -
+  have atm_of_N\<^sub>0_iff: \<open>atm_of x \<in> set N\<^sub>0 \<longleftrightarrow>
+         x \<in> (- literal_of_nat \<circ>\<circ> op *) 2 ` set N\<^sub>0 \<or> x \<in> (literal_of_nat \<circ>\<circ> op *) 2 ` set N\<^sub>0\<close>
+    for x N\<^sub>0
+    by (cases x)  auto
   have is_N\<^sub>1_add: \<open>twl_array_code_ops.is_N\<^sub>1 N\<^sub>0 (A + B) \<longleftrightarrow> set_mset A \<subseteq> set_mset (twl_array_code_ops.N\<^sub>1 N\<^sub>0)\<close>
     if \<open>twl_array_code_ops.is_N\<^sub>1 N\<^sub>0 B\<close> for A B N\<^sub>0
     using that unfolding twl_array_code_ops.is_N\<^sub>1_def by auto
@@ -346,10 +344,15 @@ proof -
     by (rule image_cong)
       (use that in \<open>auto simp del: literal_of_nat.simps simp: nat_of_uint32_uint32_of_nat_id
   upperN_def\<close>)
-
-  have H2: \<open>(\<lambda>x. literal_of_nat (nat_of_uint32 (uint32_of_nat (nat_of_lit x)))) ` set N\<^sub>0 =
-        id ` set N\<^sub>0\<close>
-    if \<open>\<forall>L\<in>set N\<^sub>0. nat_of_lit L < upperN\<close> for N\<^sub>0
+  have H2: \<open>(\<lambda>x. literal_of_nat (nat_of_uint32 (uint32_of_nat (2 * x)))) ` set N\<^sub>0 =
+        (literal_of_nat o (op * 2)) ` set N\<^sub>0\<close>
+    if \<open>\<forall>L\<in>set N\<^sub>0.  L < upperN div 2\<close> for N\<^sub>0
+    by (rule image_cong)
+       (use that in \<open>auto simp del: literal_of_nat.simps simp: nat_of_uint32_uint32_of_nat_id
+  upperN_def\<close>)
+  have H2': \<open>(\<lambda>x. -literal_of_nat (nat_of_uint32 (uint32_of_nat (2 * x)))) ` set N\<^sub>0 =
+        (- literal_of_nat o (op * 2)) ` set N\<^sub>0\<close>
+    if \<open>\<forall>L\<in>set N\<^sub>0. L < upperN div 2\<close> for N\<^sub>0
     by (rule image_cong)
       (use that in \<open>auto simp del: literal_of_nat.simps simp: nat_of_uint32_uint32_of_nat_id
   upperN_def\<close>)
@@ -357,24 +360,28 @@ proof -
     using upper upperN
   proof (induction N arbitrary: N\<^sub>0)
     case Nil
-    then show ?case by (auto simp: extract_lits_cls_def extract_lits_clss_def twl_array_code_ops.is_N\<^sub>1_def
-          twl_array_code_ops.N\<^sub>1_def in_lits_of_atms_of_m_ain_atms_of_iff twl_array_code_ops.N\<^sub>0''_def
-          twl_array_code_ops.N\<^sub>0'_def atm_of_eq_atm_of H1 H2
+    then show ?case by (auto simp: extract_atms_cls_def extract_atms_clss_def twl_array_code_ops.is_N\<^sub>1_def
+          twl_array_code_ops.N\<^sub>1_def in_all_lits_of_m_ain_atms_of_iff twl_array_code_ops.N\<^sub>0''_def
+          twl_array_code_ops.N\<^sub>0'_def atm_of_eq_atm_of H1 H2 H2' all_lits_of_atms_m_all_lits_of_m
+          N\<^sub>0_of_atms_def atm_of_N\<^sub>0_iff
           simp del: nat_of_lit.simps literal_of_nat.simps)
   next
     case (Cons C Cs N\<^sub>0) note IH = this(1) and H=this(2-)
-    then have \<open>\<forall>L\<in>set (extract_lits_cls C N\<^sub>0). nat_of_lit L < upperN\<close>
-      by (auto dest!: in_extract_lits_clsD simp: nat_of_lit_upperN_nat_of_lit_uminus_upperN)
+    have \<open>2 * L < upperN \<longleftrightarrow> L < upperN div 2\<close> for L
+      by (auto simp: upperN_def)
+    then have \<open>\<forall>L\<in>set (extract_atms_cls C N\<^sub>0). L < upperN div 2\<close>
+      using Cons
+      by (auto dest!: in_extract_atms_clsD simp: nat_of_lit_upperN_nat_of_lit_uminus_upperN)
     then show ?case
-      using IH[of \<open>extract_lits_cls C N\<^sub>0\<close>, unfolded twl_array_code_ops.is_N\<^sub>1_def] H
-      by (simp add: lits_of_atms_of_mm_add_mset twl_array_code_ops.is_N\<^sub>1_def
-          lits_of_atms_of_m_extract_lits_cls ac_simps comp_def)
+      using IH[of \<open>extract_atms_cls C N\<^sub>0\<close>, unfolded twl_array_code_ops.is_N\<^sub>1_def] H
+      by (simp add: all_lits_of_mm_add_mset twl_array_code_ops.is_N\<^sub>1_def
+          all_lits_of_m_extract_atms_cls ac_simps comp_def)
   qed
 qed
 
 fun correct_watching_init :: \<open>nat literal multiset \<Rightarrow> nat twl_st_wl \<Rightarrow> bool\<close> where
   \<open>correct_watching_init N\<^sub>1 (M, N, U, D, NP, UP, Q, W) \<longleftrightarrow>
-    (\<forall>L \<in># lits_of_atms_of_m N\<^sub>1. mset (W L) = clause_to_update L (M, N, U, D, NP, UP, {#}, {#}))\<close>
+    (\<forall>L \<in># all_lits_of_m N\<^sub>1. mset (W L) = clause_to_update L (M, N, U, D, NP, UP, {#}, {#}))\<close>
 
 
 lemma clause_to_update_append: \<open>N \<noteq> [] \<Longrightarrow> clause_to_update La (M, N @ [C], U, D, NP, UP, WS, Q) =
@@ -389,27 +396,28 @@ definition HH :: \<open>nat literal multiset \<Rightarrow> (nat twl_st_wl \<time
                M = M' \<and> N = N' \<and> U = U' \<and> D = D' \<and> NP = NP' \<and> UP = UP' \<and> Q = Q' \<and> WS = {#} \<and>
                (* U = length N - 1 \<and> *) UP = {#} \<and> N \<noteq> [] \<and>
                correct_watching_init N\<^sub>1 (M', N', U', D', NP', UP', Q', WS') \<and>
-               set_mset (lits_of_atms_of_mm (mset `# mset (tl N) + NP)) \<subseteq> set_mset N\<^sub>1 \<and>
+               set_mset (all_lits_of_mm (mset `# mset (tl N) + NP)) \<subseteq> set_mset N\<^sub>1 \<and>
                (\<forall>L \<in> lits_of_l M. {#L#} \<in># NP) \<and>
                (\<forall>L \<in> set M. \<exists>K. L = Propagated K 0)}\<close>
 
+context twl_array_code
+begin
 lemma literals_are_in_N\<^sub>0_add_mset:
-  \<open>twl_array_code_ops.literals_are_in_N\<^sub>0 N\<^sub>0 (add_mset L M) \<longleftrightarrow>
-   twl_array_code_ops.literals_are_in_N\<^sub>0 N\<^sub>0 M \<and>
+  \<open>literals_are_in_N\<^sub>0 (add_mset L M) \<longleftrightarrow>
+   literals_are_in_N\<^sub>0 M \<and>
       (L \<in> literal_of_nat ` nat_of_uint32 ` set N\<^sub>0 \<or> -L \<in> literal_of_nat ` nat_of_uint32 ` set N\<^sub>0)\<close>
   by (auto simp: twl_array_code_ops.N\<^sub>1_def twl_array_code_ops.N\<^sub>0''_def twl_array_code_ops.N\<^sub>0'_def
-      twl_array_code_ops.literals_are_in_N\<^sub>0_def image_image lits_of_atms_of_m_add_mset uminus_lit_swap
+      twl_array_code_ops.literals_are_in_N\<^sub>0_def image_image all_lits_of_m_add_mset uminus_lit_swap
         simp del: literal_of_nat.simps)
 
 lemma init_dt_step_wl_init_dt_step_l:
-  fixes N\<^sub>0 :: \<open>uint32 list\<close>
   defines \<open>N\<^sub>0' \<equiv> map nat_of_uint32 N\<^sub>0\<close>
   defines \<open>N\<^sub>1 \<equiv> mset (map literal_of_nat N\<^sub>0') + mset (map (uminus o literal_of_nat) N\<^sub>0')\<close>
   assumes
     \<open>(S', S) \<in> HH N\<^sub>1\<close> and
-    \<open>twl_array_code_ops.literals_are_in_N\<^sub>0 N\<^sub>0 (mset C)\<close> and
+    \<open>literals_are_in_N\<^sub>0 (mset C)\<close> and
     \<open>distinct C\<close>
-  shows \<open>init_dt_step_wl N\<^sub>0 C S' \<le> \<Down> (HH N\<^sub>1) (init_dt_step_l C S)\<close>
+  shows \<open>init_dt_step_wl C S' \<le> \<Down> (HH N\<^sub>1) (init_dt_step_l C S)\<close>
 proof -
   have val: \<open>(val, val') \<in> \<langle>Id\<rangle>option_rel\<close> if \<open>val = val'\<close> for val val'
     using that by auto
@@ -430,13 +438,13 @@ proof -
     if \<open>C \<noteq> []\<close>
     using assms(3-) that
     by (cases C) (auto simp: HH_def correct_watching.simps clause_to_update_def
-        lits_of_atms_of_mm_add_mset lits_of_atms_of_m_add_mset twl_array_code_ops.N\<^sub>1_def
+        all_lits_of_mm_add_mset all_lits_of_m_add_mset twl_array_code_ops.N\<^sub>1_def
         twl_array_code_ops.N\<^sub>0''_def twl_array_code_ops.N\<^sub>0'_def
         twl_array_code_ops.literals_are_in_N\<^sub>0_def clauses_def mset_take_mset_drop_mset')
   have hd_tl_C: \<open>hd (tl C) \<in> snd ` (\<lambda>L. (nat_of_lit L, L)) ` set_mset (twl_array_code_ops.N\<^sub>1 N\<^sub>0)\<close>
     if \<open>C \<noteq> []\<close> and \<open>tl C \<noteq> []\<close>
     using assms(3-) that by (cases C; cases \<open>tl C\<close>) (auto simp: HH_def Let_def clause_to_update_append
-        clauses_def mset_take_mset_drop_mset' image_image lits_of_atms_of_m_add_mset
+        clauses_def mset_take_mset_drop_mset' image_image all_lits_of_m_add_mset
         twl_array_code_ops.literals_are_in_N\<^sub>0_def)
 
   have add_unit_clause_ref:
@@ -460,7 +468,7 @@ proof -
     for M SM N SN U SU D SD NP SNP UP SUP' W Q M' SM' N' SN' U' SU' D' SD' NP' SNP' UP'
       SUP'' W' Q'
     using assms(3-) that hd_C by (cases C)
-      (auto simp: HH_def lits_of_atms_of_mm_add_mset lits_of_atms_of_m_add_mset)
+      (auto simp: HH_def all_lits_of_mm_add_mset all_lits_of_m_add_mset)
   have add_unit_clause_confl_ref:
     \<open>((M', N', U', Some (mset C), add_mset {#hd C#} NP', UP', {#}, Q'),
        M, N, U, Some (mset C), add_mset {#hd C#} NP, UP, {#}, {#}) \<in> HH N\<^sub>1\<close>
@@ -483,7 +491,7 @@ proof -
     for M SM N SN U SU D SD NP SNP UP SUP' W Q M' SM' N' SN' U' SU' D' SD' NP' SNP' UP'
       SUP'' W' Q'
     using that assms(2-) hd_C by (cases C)
-        (auto simp: HH_def lits_of_atms_of_mm_add_mset lits_of_atms_of_m_add_mset)
+        (auto simp: HH_def all_lits_of_mm_add_mset all_lits_of_m_add_mset)
   have add_nonunit_clause_ref:
    \<open>SUP' = (W, Q) \<Longrightarrow>
     SNP = (UP, SUP') \<Longrightarrow>
@@ -510,8 +518,8 @@ proof -
     using assms(3-)
     apply (cases C; cases \<open>tl C\<close>)
        apply ((fast; fail)+ )[3]
-    by (auto simp: HH_def Let_def clause_to_update_append lits_of_atms_of_m_add_mset
-        lits_of_atms_of_mm_add_mset literals_are_in_N\<^sub>0_add_mset
+    by (auto simp: HH_def Let_def clause_to_update_append all_lits_of_m_add_mset
+        all_lits_of_mm_add_mset literals_are_in_N\<^sub>0_add_mset
         twl_array_code_ops.literals_are_in_N\<^sub>0_def)[]
   have add_unit_clause_conflict:
     \<open>SUP' = (W, Q) \<Longrightarrow>
@@ -535,8 +543,8 @@ proof -
     for M SM N SN U SU D SD NP SNP UP SUP' W Q M' SM' N' SN' U' SU' D' SD' NP' SNP' UP'
       SUP'' W' Q' E E'
     using assms(3-)
-    by (cases C; cases \<open>tl C\<close>) (auto simp: HH_def lits_of_atms_of_mm_add_mset
-        lits_of_atms_of_m_add_mset twl_array_code_ops.literals_are_in_N\<^sub>0_def)
+    by (cases C; cases \<open>tl C\<close>) (auto simp: HH_def all_lits_of_mm_add_mset
+        all_lits_of_m_add_mset twl_array_code_ops.literals_are_in_N\<^sub>0_def)
   have add_nonunit_clause_conflict:
     \<open>SUP' = (W, Q) \<Longrightarrow>
     SNP = (UP, SUP') \<Longrightarrow>
@@ -568,8 +576,8 @@ proof -
     using assms(3-)
     by (cases C; cases \<open>tl C\<close>)
      (auto simp: HH_def Let_def clause_to_update_append
-        lits_of_atms_of_m_add_mset
-        lits_of_atms_of_mm_add_mset literals_are_in_N\<^sub>0_add_mset
+        all_lits_of_m_add_mset
+        all_lits_of_mm_add_mset literals_are_in_N\<^sub>0_add_mset
         twl_array_code_ops.literals_are_in_N\<^sub>0_def)
 
   show ?thesis
@@ -583,7 +591,7 @@ proof -
     subgoal by (rule hd_C) assumption
     subgoal by (auto simp: HH_def)
     subgoal by (cases C)
-        (auto simp: HH_def lits_of_atms_of_mm_add_mset lits_of_atms_of_m_add_mset)
+        (auto simp: HH_def all_lits_of_mm_add_mset all_lits_of_m_add_mset)
     subgoal by (auto simp only: HH_def)
     subgoal by (rule add_unit_clause_ref) assumption+
     subgoal by (rule add_unit_clause_confl_ref)
@@ -623,7 +631,7 @@ lemma init_dt_wl_init_dt_l:
 
 abbreviation twl_code_array_literals_are_N\<^sub>0 where
   \<open>twl_code_array_literals_are_N\<^sub>0 N\<^sub>0 S \<equiv>
-     twl_array_code_ops.is_N\<^sub>1 N\<^sub>0 (lits_of_atms_of_mm (cdcl\<^sub>W_restart_mset.clauses (state\<^sub>W_of (twl_st_of_wl None S))))\<close>
+     twl_array_code_ops.is_N\<^sub>1 N\<^sub>0 (all_lits_of_mm (cdcl\<^sub>W_restart_mset.clauses (state\<^sub>W_of (twl_st_of_wl None S))))\<close>
 
 fun get_clauses_wl :: "'v twl_st_wl \<Rightarrow> 'v clauses_l" where
   \<open>get_clauses_wl (M, N, U, D, NP, UP, WS, Q) = N\<close>
@@ -631,10 +639,10 @@ fun get_clauses_wl :: "'v twl_st_wl \<Rightarrow> 'v clauses_l" where
 fun get_learned_wl :: "'v twl_st_wl \<Rightarrow> nat" where
   \<open>get_learned_wl (M, N, U, D, NP, UP, WS, Q) = U\<close>
 
-lemma lits_of_atms_of_mm_in_lits_of_atms_of_m_in_iff:
-  \<open>set_mset (lits_of_atms_of_mm (mset `# mset CS)) \<subseteq> A \<longleftrightarrow>
-    (\<forall>C\<in>set CS. set_mset (lits_of_atms_of_m (mset C)) \<subseteq> A)\<close>
-  by (auto simp: lits_of_atms_of_mm_def lits_of_atms_of_m_def)
+lemma all_lits_of_mm_in_all_lits_of_m_in_iff:
+  \<open>set_mset (all_lits_of_mm (mset `# mset CS)) \<subseteq> A \<longleftrightarrow>
+    (\<forall>C\<in>set CS. set_mset (all_lits_of_m (mset C)) \<subseteq> A)\<close>
+  by (auto simp: all_lits_of_mm_def all_lits_of_m_def)
 
 definition get_unit_learned :: "'v twl_st_wl \<Rightarrow> 'v clauses" where
   \<open>get_unit_learned = (\<lambda>(M, N, U, D, NP, UP, Q, W). UP)\<close>
@@ -644,8 +652,8 @@ definition get_unit_init_clss :: "'v twl_st_wl \<Rightarrow> 'v clauses" where
 
 lemma init_dt_init_dt_l_full:
   fixes S :: \<open>nat twl_st_wl\<close> and CS
-  defines \<open>N\<^sub>0 \<equiv> map (uint32_of_nat o nat_of_lit) (extract_lits_clss CS [])\<close>
-  defines \<open>N\<^sub>0' \<equiv> map nat_of_uint32 N\<^sub>0\<close>
+  defines \<open>N\<^sub>0 \<equiv> map uint32_of_nat (extract_atms_clss CS [])\<close>
+  defines \<open>N\<^sub>0' \<equiv> (extract_atms_clss CS [])\<close>
   defines \<open>N\<^sub>1 \<equiv> mset (map literal_of_nat N\<^sub>0') + mset (map (uminus o literal_of_nat) N\<^sub>0')\<close>
   assumes
     dist: \<open>\<forall>C \<in> set CS. distinct C\<close> and
@@ -659,7 +667,7 @@ lemma init_dt_init_dt_l_full:
     stgy_invs: \<open>twl_stgy_invs (twl_st_of_wl None S)\<close> and
     watch: \<open>correct_watching_init N\<^sub>1 S\<close> and
     clss: \<open>get_clauses_wl S \<noteq> []\<close> and
-    S_N\<^sub>1: \<open>set_mset (lits_of_atms_of_mm (cdcl\<^sub>W_restart_mset.clauses
+    S_N\<^sub>1: \<open>set_mset (all_lits_of_mm (cdcl\<^sub>W_restart_mset.clauses
       (state\<^sub>W_of (twl_st_of None (st_l_of_wl None S))))) \<subseteq> set_mset N\<^sub>1\<close> and
     no_learned: \<open>get_unit_learned S = {#}\<close> and
     confl_in_clss: \<open>get_conflict_wl S \<noteq> None \<longrightarrow> the (get_conflict_wl S) \<in># mset `# mset CS\<close> and
@@ -668,7 +676,7 @@ lemma init_dt_init_dt_l_full:
     upper: \<open>\<forall>C\<in>set CS. \<forall>L\<in>set C. nat_of_lit L < upperN\<close>
   shows
     \<open>init_dt_wl N\<^sub>0 CS S \<le> SPEC(\<lambda>T.
-       twl_array_code_ops.is_N\<^sub>1 N\<^sub>0 (lits_of_atms_of_mm (mset `# mset CS +
+       twl_array_code_ops.is_N\<^sub>1 N\<^sub>0 (all_lits_of_mm (mset `# mset CS +
           cdcl\<^sub>W_restart_mset.clauses (state\<^sub>W_of (twl_st_of None (st_l_of_wl None S))))) \<and>
        twl_struct_invs (twl_st_of_wl None T) \<and> twl_stgy_invs (twl_st_of_wl None T) \<and>
        additional_WS_invs (st_l_of_wl None T) \<and>
@@ -722,26 +730,26 @@ proof -
     apply (intro conjI)
     using init apply (simp_all add: count_decided_def)
     done
-   have CS_N\<^sub>1: \<open>\<forall>C\<in>set CS. twl_array_code_ops.literals_are_in_N\<^sub>0 N\<^sub>0 (mset C)\<close>
-    using is_N\<^sub>1_extract_lits_clss[of \<open>[]\<close> CS] upper unfolding N\<^sub>1_def N\<^sub>0_def
+   have CS_N\<^sub>1: \<open>\<forall>C\<in>set CS. twl_array_code_ops.literals_are_in_N\<^sub>0 (N\<^sub>0_of_atms N\<^sub>0) (mset C)\<close>
+    using is_N\<^sub>1_extract_atms_clss[of \<open>[]\<close> CS] upper unfolding N\<^sub>1_def N\<^sub>0_def
       twl_array_code_ops.is_N\<^sub>1_def twl_array_code_ops.N\<^sub>1_def twl_array_code_ops.N\<^sub>0''_def
       twl_array_code_ops.N\<^sub>0'_def twl_array_code_ops.literals_are_in_N\<^sub>0_def
-    by (simp del: literal_of_nat.simps add: lits_of_atms_of_mm_in_lits_of_atms_of_m_in_iff[symmetric])
-  have is_N\<^sub>1: \<open>twl_array_code_ops.is_N\<^sub>1 N\<^sub>0 (lits_of_atms_of_mm (mset `# mset CS))\<close>
-    using is_N\<^sub>1_extract_lits_clss[of \<open>[]\<close> CS] upper unfolding N\<^sub>1_def N\<^sub>0_def
+    by (simp del: literal_of_nat.simps add: all_lits_of_mm_in_all_lits_of_m_in_iff[symmetric])
+  have is_N\<^sub>1: \<open>twl_array_code_ops.is_N\<^sub>1 N\<^sub>0 (all_lits_of_mm (mset `# mset CS))\<close>
+    using is_N\<^sub>1_extract_atms_clss[of \<open>[]\<close> CS] upper unfolding N\<^sub>1_def N\<^sub>0_def
       twl_array_code_ops.is_N\<^sub>1_def twl_array_code_ops.N\<^sub>1_def twl_array_code_ops.N\<^sub>0''_def
       twl_array_code_ops.N\<^sub>0'_def twl_array_code_ops.literals_are_in_N\<^sub>0_def
-    by (simp del: literal_of_nat.simps add: lits_of_atms_of_mm_in_lits_of_atms_of_m_in_iff[symmetric])
+    by (simp del: literal_of_nat.simps add: all_lits_of_mm_in_all_lits_of_m_in_iff[symmetric])
   have Un_eq_iff_subset: \<open>A \<union> B = A \<longleftrightarrow> B \<subseteq> A\<close> for A B
     by blast
-  have [simp]: \<open>twl_array_code_ops.is_N\<^sub>1 N\<^sub>0 (A + lits_of_atms_of_mm B) \<longleftrightarrow>
-       set_mset (lits_of_atms_of_mm B) \<subseteq> set_mset N\<^sub>1\<close>
+  have [simp]: \<open>twl_array_code_ops.is_N\<^sub>1 N\<^sub>0 (A + all_lits_of_mm B) \<longleftrightarrow>
+       set_mset (all_lits_of_mm B) \<subseteq> set_mset N\<^sub>1\<close>
     if \<open>twl_array_code_ops.is_N\<^sub>1 N\<^sub>0 A\<close> for A B
     using that by (simp add: twl_array_code_ops.is_N\<^sub>1_def twl_array_code_ops.literals_are_in_N\<^sub>0_def
         Un_eq_iff_subset N\<^sub>0_N\<^sub>1)
-  have CS_N\<^sub>1': \<open>set_mset (lits_of_atms_of_mm (mset `# mset CS)) \<subseteq> set_mset N\<^sub>1\<close>
-    using is_N\<^sub>1 unfolding twl_array_code_ops.is_N\<^sub>1_def by (clarsimp simp: HH_def lits_of_atms_of_mm_union N\<^sub>0_N\<^sub>1)
-  have \<open>set_mset (lits_of_atms_of_mm (cdcl\<^sub>W_restart_mset.clauses
+  have CS_N\<^sub>1': \<open>set_mset (all_lits_of_mm (mset `# mset CS)) \<subseteq> set_mset N\<^sub>1\<close>
+    using is_N\<^sub>1 unfolding twl_array_code_ops.is_N\<^sub>1_def by (clarsimp simp: HH_def all_lits_of_mm_union N\<^sub>0_N\<^sub>1)
+  have \<open>set_mset (all_lits_of_mm (cdcl\<^sub>W_restart_mset.clauses
       (state\<^sub>W_of (twl_st_of None (st_l_of_wl None S))))) \<subseteq>
    set_mset N\<^sub>1\<close>
     using S_N\<^sub>1 unfolding twl_array_code_ops.is_N\<^sub>1_def
@@ -760,7 +768,7 @@ proof -
     subgoal using CS_N\<^sub>1 by auto
     subgoal using dist .
     subgoal using is_N\<^sub>1 CS_N\<^sub>1' S_N\<^sub>1 unfolding conc_fun_RES
-      by (clarsimp simp: HH_def lits_of_atms_of_mm_union mset_take_mset_drop_mset'
+      by (clarsimp simp: HH_def all_lits_of_mm_union mset_take_mset_drop_mset'
           clauses_def get_unit_learned_def get_unit_init_clss_def N\<^sub>1_def N\<^sub>0'_def
           simp del: literal_of_nat.simps)
     done
@@ -769,7 +777,7 @@ qed
 lemma init_dt_init_dt_l:
   fixes CS
   defines \<open>S \<equiv> ([], [[]], 0, None, {#}, {#}, {#}, \<lambda>_. [])\<close>
-  defines \<open>N\<^sub>0 \<equiv> map (uint32_of_nat o nat_of_lit) (extract_lits_clss CS [])\<close>
+  defines \<open>N\<^sub>0 \<equiv> map (uint32_of_nat) (extract_atms_clss CS [])\<close>
   defines \<open>N\<^sub>0' \<equiv> map nat_of_uint32 N\<^sub>0\<close>
   defines \<open>N\<^sub>1 \<equiv> mset (map literal_of_nat N\<^sub>0') + mset (map (uminus o literal_of_nat) N\<^sub>0')\<close>
   assumes
@@ -779,7 +787,7 @@ lemma init_dt_init_dt_l:
     upper: \<open>\<forall>C\<in>set CS. \<forall>L\<in>set C. nat_of_lit L < upperN\<close>
   shows
     \<open>init_dt_wl N\<^sub>0 CS S \<le> SPEC(\<lambda>S.
-       twl_array_code_ops.is_N\<^sub>1 N\<^sub>0 (lits_of_atms_of_mm (mset `# mset CS)) \<and>
+       twl_array_code_ops.is_N\<^sub>1 N\<^sub>0 (all_lits_of_mm (mset `# mset CS)) \<and>
        twl_struct_invs (twl_st_of_wl None S) \<and> twl_stgy_invs (twl_st_of_wl None S) \<and>
        correct_watching S \<and>
        additional_WS_invs (st_l_of_wl None S) \<and>
@@ -803,7 +811,7 @@ proof -
     stgy_invs: \<open>twl_stgy_invs (twl_st_of_wl None S)\<close> and
     watch: \<open>correct_watching_init N\<^sub>1 S\<close> and
     clss: \<open>get_clauses_wl S \<noteq> []\<close> and
-    S_N\<^sub>1: \<open>set_mset (lits_of_atms_of_mm (cdcl\<^sub>W_restart_mset.clauses
+    S_N\<^sub>1: \<open>set_mset (all_lits_of_mm (cdcl\<^sub>W_restart_mset.clauses
       (state\<^sub>W_of (twl_st_of None (st_l_of_wl None S))))) \<subseteq> set_mset N\<^sub>1\<close> and
     no_learned: \<open>(\<lambda>(M, N, U, D, NP, UP, Q, W). UP) S = {#}\<close> and
     learned_nil: \<open>get_unit_learned S = {#}\<close> and
@@ -835,10 +843,10 @@ proof -
           Pos (atm_of (literal_of_nat xa)) \<in> literal_of_nat ` set N\<^sub>0' \<or>
           Neg (atm_of (literal_of_nat xa)) \<in> literal_of_nat ` set N\<^sub>0'\<close> for xa
     by (cases \<open>literal_of_nat xa\<close>) (auto split: if_splits)
-  have \<open>set_mset N\<^sub>1 \<subseteq> set_mset (lits_of_atms_of_m N\<^sub>1)\<close>
-    by (fastforce simp: lits_of_atms_of_m_def N\<^sub>1_def image_image uminus_lit_swap)
-  then have [simp]: \<open>set_mset (lits_of_atms_of_m N\<^sub>1) = set_mset N\<^sub>1\<close>
-    by (fastforce simp: lits_of_atms_of_m_def N\<^sub>1_def image_image uminus_lit_swap
+  have \<open>set_mset N\<^sub>1 \<subseteq> set_mset (all_lits_of_m N\<^sub>1)\<close>
+    by (fastforce simp: all_lits_of_m_def N\<^sub>1_def image_image uminus_lit_swap)
+  then have [simp]: \<open>set_mset (all_lits_of_m N\<^sub>1) = set_mset N\<^sub>1\<close>
+    by (fastforce simp: all_lits_of_m_def N\<^sub>1_def image_image uminus_lit_swap
         simp del: literal_of_nat.simps dest: H)
   show ?thesis
     apply (rule order.trans)
@@ -875,7 +883,7 @@ definition SAT :: \<open>nat clauses \<Rightarrow> nat cdcl\<^sub>W_restart_mset
 definition SAT_wl :: \<open>nat clauses_l \<Rightarrow> nat twl_st_wl nres\<close> where
   \<open>SAT_wl CS = do{
     let n = length CS;
-    let N\<^sub>0 = map (uint32_of_nat o nat_of_lit) (extract_lits_clss CS []);
+    let N\<^sub>0 = map (uint32_of_nat o nat_of_lit) (extract_atms_clss CS []);
     let S = twl_array_code_ops.init_state_wl N\<^sub>0;
     T \<leftarrow> init_dt_wl N\<^sub>0 CS S;
     if get_conflict_wl T = None
@@ -1108,7 +1116,7 @@ lemma initialise_VMTF_href:
 definition SAT_wl' :: \<open>nat clauses_l \<Rightarrow> bool nres\<close> where
   \<open>SAT_wl' CS = do{
     let n = length CS;
-    let N\<^sub>0 = map_uint32_of_lit (extract_lits_clss CS []);
+    let N\<^sub>0 = map_uint32_of_lit (extract_atms_clss CS []);
     ASSERT(twl_array_code N\<^sub>0);
     let S = twl_array_code_ops.init_state_wl N\<^sub>0;
     T \<leftarrow> init_dt_wl N\<^sub>0 CS S;
@@ -1464,7 +1472,7 @@ unfolded twl_array_code_ops.twl_st_l_trail_assn_def]
 sepref_definition SAT_wl_code
   is \<open>SAT_wl'\<close>
   :: \<open>(list_assn (list_assn unat_lit_assn))\<^sup>k \<rightarrow>\<^sub>a bool_assn\<close>
-  unfolding SAT_wl'_def HOL_list.fold_custom_empty extract_lits_cls'_extract_lits_cls[symmetric]
+  unfolding SAT_wl'_def HOL_list.fold_custom_empty extract_atms_cls'_extract_atms_cls[symmetric]
     PR_CONST_def get_conflict_wl_is_None
   supply twl_array_code_ops.get_conflict_wl_is_None_code_refine[sepref_fr_rules]
     supply twl_array_code.init_dt_wl_code_refine'[sepref_fr_rules]
@@ -1519,14 +1527,14 @@ proof -
     by (subst (2) append_take_drop_id[symmetric, of \<open>tl af\<close> ag], subst mset_append)
       (auto simp: drop_Suc)
   have if_no_confl_ref:
-    \<open>(if get_conflict_wl S\<^sub>0 = None then twl_array_code.cdcl_twl_stgy_prog_wl_D (map (uint32_of_nat \<circ> nat_of_lit) (extract_lits_clss CS' [])) S\<^sub>0 else RETURN S\<^sub>0)
+    \<open>(if get_conflict_wl S\<^sub>0 = None then twl_array_code.cdcl_twl_stgy_prog_wl_D (map (uint32_of_nat \<circ> nat_of_lit) (extract_atms_clss CS' [])) S\<^sub>0 else RETURN S\<^sub>0)
     \<le> \<Down> TWL_to_clauses_state_conv
         (SPEC (\<lambda>U. full cdcl\<^sub>W_restart_mset.cdcl\<^sub>W_stgy (CDCL_Two_Watched_Literals_List_Watched_Init_Trail_Code.init_state CS) U \<or>
                     cdcl\<^sub>W_restart_mset.clauses U = CS \<and> learned_clss U = {#} \<and> conflicting U \<noteq> None \<and> backtrack_lvl U = 0 \<and> cdcl\<^sub>W_restart_mset.cdcl\<^sub>W_all_struct_inv U))\<close>
     if
       CS_p: \<open>Multiset.Ball CS distinct_mset \<and> (\<forall>C\<in>#CS. 1 \<le> size C) \<and> (\<forall>C\<in>#CS. \<not> tautology C) \<and> (\<forall>C\<in>#CS. \<forall>L\<in>#C. nat_of_lit L < upperN)\<close> and
       CS'_CS: \<open>(CS', CS) \<in> list_mset_rel O \<langle>list_mset_rel\<rangle>mset_rel\<close> and
-      N\<^sub>1: \<open>twl_array_code_ops.is_N\<^sub>1 (map (uint32_of_nat \<circ> nat_of_lit) (extract_lits_clss CS' [])) (lits_of_atms_of_mm (mset `# mset CS'))\<close> and
+      N\<^sub>1: \<open>twl_array_code_ops.is_N\<^sub>1 (map (uint32_of_nat \<circ> nat_of_lit) (extract_atms_clss CS' [])) (all_lits_of_mm (mset `# mset CS'))\<close> and
       struct_invs: \<open>twl_struct_invs (twl_st_of_wl None S\<^sub>0)\<close> and
       stgy_invs: \<open>twl_stgy_invs (twl_st_of_wl None S\<^sub>0)\<close> and
       corr_w: \<open>correct_watching S\<^sub>0\<close> and
@@ -1592,15 +1600,15 @@ proof -
        (state\<^sub>W_of (twl_st_of None (st_l_of_wl None S\<^sub>0)))\<close>
       using 0 by (auto simp: S\<^sub>0 CS mset_take_mset_drop_mset' N_NP init_state_def)
 
-    have \<open>twl_array_code (map (uint32_of_nat \<circ> nat_of_lit) (extract_lits_clss CS' []))\<close>
+    have \<open>twl_array_code (map (uint32_of_nat \<circ> nat_of_lit) (extract_atms_clss CS' []))\<close>
       unfolding twl_array_code_def
     proof
       fix L
-      assume \<open>L \<in> set (map (uint32_of_nat \<circ> nat_of_lit) (extract_lits_clss CS' []))\<close>
+      assume \<open>L \<in> set (map (uint32_of_nat \<circ> nat_of_lit) (extract_atms_clss CS' []))\<close>
       then obtain x where
         L: \<open>L = uint32_of_nat (nat_of_lit x)\<close> and
         xa: \<open>(\<exists>xa\<in>set CS'. x \<in> set xa) \<or> (\<exists>xa\<in>set CS'. - x \<in> set xa)\<close>
-        by (clarsimp dest!: in_extract_lits_clssD simp: upperN_def nat_of_uint32_uint32_of_nat_id)
+        by (clarsimp dest!: in_extract_atms_clssD simp: upperN_def nat_of_uint32_uint32_of_nat_id)
       have \<open>\<forall>C\<in>#CS. \<forall>L\<in>#C. nat_of_lit L < upperN\<close>
         using CS_p by auto
       then have \<open>nat_of_lit x < upperN\<close>
@@ -1608,17 +1616,17 @@ proof -
         by auto
       then show \<open> nat_of_uint32 L < upperN\<close>
         using L
-        by (clarsimp dest!: in_extract_lits_clssD simp: upperN_def nat_of_uint32_uint32_of_nat_id)
+        by (clarsimp dest!: in_extract_atms_clssD simp: upperN_def nat_of_uint32_uint32_of_nat_id)
     qed
-    then have 2: \<open>twl_array_code.cdcl_twl_stgy_prog_wl_D (map (uint32_of_nat o nat_of_lit) (extract_lits_clss CS' [])) S\<^sub>0
+    then have 2: \<open>twl_array_code.cdcl_twl_stgy_prog_wl_D (map (uint32_of_nat o nat_of_lit) (extract_atms_clss CS' [])) S\<^sub>0
        \<le> SPEC (\<lambda>T. full cdcl\<^sub>W_restart_mset.cdcl\<^sub>W_stgy
                      (state\<^sub>W_of (twl_st_of None (st_l_of_wl None S\<^sub>0)))
                      (state\<^sub>W_of (twl_st_of None (st_l_of_wl None T))))\<close>
       using twl_array_code.cdcl_twl_stgy_prog_wl_spec_final2[of
-              \<open>(map (uint32_of_nat o nat_of_lit) (extract_lits_clss CS' []))\<close> S\<^sub>0]  CS_p N\<^sub>1
+              \<open>(map (uint32_of_nat o nat_of_lit) (extract_atms_clss CS' []))\<close> S\<^sub>0]  CS_p N\<^sub>1
             struct_invs stgy_invs corr_w add_invs clss 1 True by auto
 
-    have \<open>twl_array_code.cdcl_twl_stgy_prog_wl_D (map (uint32_of_nat o nat_of_lit) (extract_lits_clss CS' [])) S\<^sub>0
+    have \<open>twl_array_code.cdcl_twl_stgy_prog_wl_D (map (uint32_of_nat o nat_of_lit) (extract_atms_clss CS' [])) S\<^sub>0
       \<le> \<Down> TWL_to_clauses_state_conv
       (SPEC (full cdcl\<^sub>W_restart_mset.cdcl\<^sub>W_stgy (init_state CS)))\<close>
       by (auto simp: TWL_to_clauses_state_conv_def conc_fun_RES rtranclp_fullI
@@ -1784,17 +1792,17 @@ proof -
   have 1: \<open>(H \<bind>
     (\<lambda>T. if get_conflict_wl T = None
           then twl_array_code.cdcl_twl_stgy_prog_wl_D
-                (map_uint32_of_lit (extract_lits_clss CS [])) T \<bind>
+                (map_uint32_of_lit (extract_atms_clss CS [])) T \<bind>
                (\<lambda>U. RETURN (get_conflict_wl U = None))
           else RETURN False)) =
     (H \<bind>
      (\<lambda>T. if get_conflict_wl T = None
            then twl_array_code.cdcl_twl_stgy_prog_wl_D
-                 (map_uint32_of_lit (extract_lits_clss CS [])) T
+                 (map_uint32_of_lit (extract_atms_clss CS [])) T
            else RETURN T)) \<bind>
     (\<lambda>T. RETURN (get_conflict_wl T = None))\<close> for H CS
     by (smt bind_cong nres_monad1 nres_monad3)
-  have SAT_wl': \<open>SAT_wl' CS = do { ASSERT (twl_array_code (map_uint32_of_lit (extract_lits_clss CS []))); T \<leftarrow> SAT_wl CS; RETURN (get_conflict_wl T = None)}\<close> for CS
+  have SAT_wl': \<open>SAT_wl' CS = do { ASSERT (twl_array_code (map_uint32_of_lit (extract_atms_clss CS []))); T \<leftarrow> SAT_wl CS; RETURN (get_conflict_wl T = None)}\<close> for CS
     unfolding SAT_wl'_def SAT_wl_def Let_def map_uint32_of_lit_def[symmetric]
     by (auto cong: bind_cong simp: 1)
   have 2: \<open>Multiset.Ball y distinct_mset \<and>
@@ -1805,7 +1813,7 @@ proof -
     using cdcl_twl_stgy_prog_wl_spec_final2[unfolded fref_def nres_rel_def] by simp
   have SAT': \<open>SAT' CS = do { ASSERT(True); T \<leftarrow> SAT CS; RETURN(conflicting T = None) } \<close> for CS
     unfolding SAT'_def by auto
-  have 3: \<open>ASSERT (twl_array_code (map_uint32_of_lit (extract_lits_clss x []))) \<le> \<Down> unit_rel (ASSERT True)\<close>
+  have 3: \<open>ASSERT (twl_array_code (map_uint32_of_lit (extract_atms_clss x []))) \<le> \<Down> unit_rel (ASSERT True)\<close>
     if \<open>(\<forall>C\<in>#y. \<forall>L\<in>#C. nat_of_lit L < upperN)\<close> and
        \<open>(x, y) \<in> list_mset_rel O \<langle>list_mset_rel\<rangle>mset_rel\<close>
        for x y
@@ -1813,11 +1821,11 @@ proof -
     unfolding twl_array_code_def
   proof
     fix L
-    assume \<open>L \<in> set (map_uint32_of_lit (extract_lits_clss x []))\<close>
+    assume \<open>L \<in> set (map_uint32_of_lit (extract_atms_clss x []))\<close>
     then obtain xa where
       L: \<open> L = uint32_of_nat (nat_of_lit xa)\<close> and
       xa: \<open>(\<exists>x\<in>set x. xa \<in> set x) \<or> (\<exists>x\<in>set x. - xa \<in> set x)\<close>
-      by (clarsimp dest!: in_extract_lits_clssD simp: upperN_def nat_of_uint32_uint32_of_nat_id
+      by (clarsimp dest!: in_extract_atms_clssD simp: upperN_def nat_of_uint32_uint32_of_nat_id
           map_uint32_of_lit_def)
     have \<open>\<forall>C\<in>#y. \<forall>L\<in># C. nat_of_lit L < upperN\<close>
       using that by auto
@@ -1829,7 +1837,7 @@ proof -
       by auto
     then show \<open>nat_of_uint32 L < upperN\<close>
       using L
-      by (clarsimp dest!: in_extract_lits_clssD simp: upperN_def nat_of_uint32_uint32_of_nat_id)
+      by (clarsimp dest!: in_extract_atms_clssD simp: upperN_def nat_of_uint32_uint32_of_nat_id)
   qed
 
   have SAT_wl'_SAT: \<open>(SAT_wl', SAT')\<in>
